zoo/language: Support strings.

lib/zoo_std/string.ml
@@ -1,0 +1,8 @@
+type t =
+  string
+
+let[@zoo.ignore] unsafe_get =
+  Stdlib.String.unsafe_get
+
+let[@zoo.ignore] equal =
+  Stdlib.String.equal
