lib/zoo_std/string.mli
@@ -1,0 +1,8 @@
+type t =
+  string
+
+val unsafe_get :
+  t -> int -> char
+
+val equal :
+  t -> t -> bool
