theories/zoo_std/string.v
@@ -1,0 +1,41 @@
+Require Import zoo.prelude.
+Require Import zoo.base.
+Require Export zoo_std.string__code.
+Require Import zoo_std.string__types.
+Require Import zoo.options.
+
+Implicit Type str : string.
+
+Definition string٠unsafe_get : val :=
+  𝗳𝘂𝗻 "t" "i" ->
+    Binop BinopStringGet "t" "i".
+
+Definition string٠equal : val :=
+  𝗳𝘂𝗻 "t1" "t2" ->
+    "t1" =ₛ "t2".
+
+Section zoo۰G.
+  Context `{zoo۰G : !ZooG Σ}.
+
+  Implicit Type Φ : val → iProp Σ.
+
+  Lemma string٠unsafe_getｰspec str i chr Φ :
+    (0 ≤ i)%Z →
+    String.get ₊i str = Some chr →
+    Φ #chr ⊢
+    WP string٠unsafe_get #str #i {{ Φ }}.
+  Proof.
+    iSteps.
+  Qed.
+
+  Lemma string٠equalｰspec str1 str2 Φ :
+    Φ #(bool_decide (str1 = str2)) ⊢
+    WP string٠equal #str1 #str2 {{ Φ }}.
+  Proof.
+    iSteps.
+  Qed.
+End zoo۰G.
+
+Require zoo_std.string__opaque.
+#[global] Opaque string٠unsafe_get.
+#[global] Opaque string٠equal.
